DeBruijnSSA/BinSyntax/Rewrite/Term/Compose.lean
@@ -1,136 +1,16 @@
 import DeBruijnSSA.BinSyntax.Rewrite.Term.Eqv
+import DeBruijnSSA.BinSyntax.Rewrite.Term.Compose.Seq
+import DeBruijnSSA.BinSyntax.Rewrite.Term.Compose.Product
 import DeBruijnSSA.BinSyntax.Typing.Term.Compose
 
 import Discretion.Utils.Quotient
+
 
 namespace BinSyntax
 
 variable [Φ: EffInstSet φ (Ty α) ε] [PartialOrder α] [SemilatticeSup ε] [OrderBot ε]
 
 namespace Term
-
-def Eqv.nil {A : Ty α} {Γ : Ctx α ε} : Eqv φ (⟨A, ⊥⟩::Γ) ⟨A, e⟩
-  := var 0 (by simp)
-
-theorem Eqv.wk0_nil {A : Ty α} {Γ : Ctx α ε}
-  : (nil : Eqv φ (⟨A, ⊥⟩::Γ) ⟨A, e⟩).wk0 (head := ⟨head, ⊥⟩) = (var 1 (by simp)) := rfl
-
-@[simp]
-theorem Eqv.wk1_nil {A : Ty α} {Γ : Ctx α ε}
-  : (nil (φ := φ) (A := A) (Γ := Γ) (e := e)).wk1 (inserted := inserted) = nil
-  := rfl
-
-@[simp]
-theorem Eqv.wk2_nil {A : Ty α} {Γ : Ctx α ε}
-  : (nil (φ := φ) (A := A) (Γ := head::Γ) (e := e)).wk2 (inserted := inserted) = nil
-  := rfl
-
-@[simp]
-theorem Eqv.subst_lift_nil {A : Ty α} {Γ : Ctx α ε} {σ : Subst.Eqv φ Γ Δ} {h}
-  : (nil : Eqv φ (⟨A, ⊥⟩::Δ) ⟨A, e⟩).subst (σ.lift h) = nil := by
-  induction σ using Quotient.inductionOn; rfl
-
-@[simp]
-theorem Eqv.wk_eff_nil {A : Ty α} {Γ : Ctx α ε} (h : lo ≤ hi)
-  : (nil (φ := φ) (A := A) (Γ := Γ)).wk_eff h = nil
-  := rfl
-
-theorem Eqv.nil_pure {A : Ty α} {Γ : Ctx α ε}
-  : (nil : Eqv φ (⟨A, ⊥⟩::Γ) ⟨A, e⟩) = nil.wk_eff bot_le
-  := rfl
-
-@[simp]
-theorem Eqv.subst0_nil_wk1 {Γ : Ctx α ε}
-  (a : Eqv φ (⟨A, ⊥⟩::Γ) V) : a.wk1.subst nil.subst0 = a
-  := by simp [nil]
-
-@[simp]
-theorem Eqv.nil_subst0 {Γ : Ctx α ε} (a : Eqv φ Γ ⟨A, ⊥⟩)
-  : (nil (e := e)).subst a.subst0 = a.wk_eff bot_le
-  := by induction a using Quotient.inductionOn; rfl
-
-@[simp]
-theorem Eqv.Pure.nil {A : Ty α} {Γ : Ctx α ε} : (nil (φ := φ) (A := A) (Γ := Γ) (e := e)).Pure
-  := ⟨Eqv.nil, rfl⟩
-
-def Eqv.seq {A B C : Ty α} {Γ : Ctx α ε}
-(a : Eqv φ ((A, ⊥)::Γ) (B, e)) (b : Eqv φ ((B, ⊥)::Γ) (C, e))
-  : Eqv φ ((A, ⊥)::Γ) (C, e)
-  := let1 a b.wk1
-
-infixl:65 " ;;' "  => Eqv.seq
-
-theorem Eqv.seq_pure {A B C : Ty α} {Γ : Ctx α ε}
-  (a : Eqv φ ((A, ⊥)::Γ) (B, ⊥)) (b : Eqv φ ((B, ⊥)::Γ) (C, ⊥)) : a ;;' b = b.wk1.subst a.subst0
-  := let1_beta_pure
-
-theorem Eqv.pure_seq {A B C : Ty α} {Γ : Ctx α ε}
-  (a : Eqv φ ((A, ⊥)::Γ) (B, ⊥)) (b : Eqv φ ((B, ⊥)::Γ) (C, e))
-  : (a.wk_eff (by simp)) ;;' b = b.wk1.subst a.subst0
-  := let1_beta
-
-theorem Eqv.wk_lift_seq {A B C : Ty α} {Δ : Ctx α ε} {ρ : Ctx.InS Γ Δ}
-  (a : Eqv φ ((A, ⊥)::Δ) (B, e)) (b : Eqv φ ((B, ⊥)::Δ) (C, e))
-  : (a ;;' b).wk (ρ.lift (le_refl _)) = (a.wk (ρ.lift (le_refl _))) ;;' (b.wk (ρ.lift (le_refl _)))
-  -- TODO: obviously true, need InS lemma
-  := by rw [seq, seq, wk_let1]; sorry
-
-theorem Eqv.wk0_seq {A B C : Ty α} {Γ : Ctx α ε}
-  (a : Eqv φ ((A, ⊥)::Γ) (B, e)) (b : Eqv φ ((B, ⊥)::Γ) (C, e))
-  : (a ;;' b).wk0 (head := ⟨head, ⊥⟩) = a.wk0 ;;' b.wk1 := by rw [seq, wk0_let1]; rfl
-
-theorem Eqv.wk1_seq {A B C : Ty α} {Γ : Ctx α ε}
-  (a : Eqv φ ((A, ⊥)::Γ) (B, e)) (b : Eqv φ ((B, ⊥)::Γ) (C, e))
-  : (a ;;' b).wk1 (inserted := inserted) = a.wk1 ;;' b.wk1 := by rw [seq, seq, wk1_let1, wk1_wk2]
-
-theorem Eqv.wk2_seq {A B C : Ty α} {Γ : Ctx α ε}
-  (a : Eqv φ ((A, ⊥)::head::Γ) (B, e)) (b : Eqv φ ((B, ⊥)::head::Γ) (C, e))
-  : (a ;;' b).wk2 (inserted := inserted) = a.wk2 ;;' b.wk2
-  := by simp only [wk2, <-Ctx.InS.lift_wk1, wk_lift_seq]
-
-@[simp]
-theorem Eqv.seq_quot {A B C : Ty α} {Γ : Ctx α ε}
-  (a : InS φ ((A, ⊥)::Γ) (B, e)) (b : InS φ ((B, ⊥)::Γ) (C, e))
-  : ⟦a⟧ ;;' ⟦b⟧ = ⟦a.seq b⟧
-  := rfl
-
-theorem Eqv.seq_wk_eff {A B C : Ty α} {Γ : Ctx α ε} {h : lo ≤ hi}
-  {a : Eqv φ ((A, ⊥)::Γ) (B, lo)} {b : Eqv φ ((B, ⊥)::Γ) (C, lo)}
-  : (a.wk_eff h) ;;' (b.wk_eff h) = (a ;;' b).wk_eff h := by
-  induction a using Quotient.inductionOn;
-  induction b using Quotient.inductionOn;
-  rfl
-
-theorem Eqv.wk_eff_seq {A B C : Ty α} {Γ : Ctx α ε} {h : lo ≤ hi}
-  {a : Eqv φ ((A, ⊥)::Γ) (B, lo)} {b : Eqv φ ((B, ⊥)::Γ) (C, lo)}
-  : (a ;;' b).wk_eff h = (a.wk_eff h) ;;' (b.wk_eff h) := seq_wk_eff.symm
-
-theorem Eqv.seq_nil {A B : Ty α} {Γ : Ctx α ε} (a : Eqv φ ((A, ⊥)::Γ) (B, e))
-  : a ;;' nil = a := let1_eta
-
-theorem Eqv.nil_seq {A B : Ty α} {Γ : Ctx α ε} (a : Eqv φ ((A, ⊥)::Γ) (B, e))
-  : nil ;;' a = a := by
-  rw [seq, <-wk_eff_nil (lo := ⊥), let1_beta, subst0_nil_wk1]
-
-theorem Eqv.seq_let1 {A B C : Ty α} {Γ : Ctx α ε}
-  (a : Eqv φ ((A, ⊥)::Γ) (B, e))
-  (b : Eqv φ ((B, ⊥)::(A, ⊥)::Γ) (C, e)) (c : Eqv φ ((C, ⊥)::Γ) (D, e))
-  : a.let1 b ;;' c = a.let1 (b ;;' c.wk1) := by rw [seq, seq, let1_let1]
-
-theorem Eqv.seq_let2 {A B C D : Ty α} {Γ : Ctx α ε}
-  (a : Eqv φ ((A, ⊥)::Γ) (B.prod B', e))
-  (b : Eqv φ ((B', ⊥)::(B, ⊥)::(A, ⊥)::Γ) (C, e)) (c : Eqv φ ((C, ⊥)::Γ) (D, e))
-  : a.let2 b ;;' c = a.let2 (b ;;' c.wk1.wk1) := by rw [seq, seq, let1_let2]
-
-theorem Eqv.let1_seq {A B C : Ty α} {Γ : Ctx α ε}
-  (a : Eqv φ ((A, ⊥)::Γ) (B, e))
-  (b : Eqv φ ((B, ⊥)::Γ) (C, e)) (c : Eqv φ ((C, ⊥)::(A, ⊥)::Γ) (D, e))
-  : let1 (a ;;' b) c = let1 a (b.wk1 ;;' c)
-  := by rw [seq, let1_let1]; rfl
-
-theorem Eqv.seq_assoc {A B C D : Ty α} {Γ : Ctx α ε}
-  (a : Eqv φ ((A, ⊥)::Γ) (B, e)) (b : Eqv φ ((B, ⊥)::Γ) (C, e)) (c : Eqv φ ((C, ⊥)::Γ) (D, e))
-  : a ;;' (b ;;' c) = (a ;;' b) ;;' c := by simp only [seq, let1_let1, wk1_let1, wk1_wk2]
 
 def Eqv.pi_l {A B : Ty α} {Γ : Ctx α ε} : Eqv φ (⟨A.prod B, ⊥⟩::Γ) ⟨A, e⟩
   := let2 nil (var 1 (by simp))
